Sangiorgi and Vignudelli's example modulo wp_flip_empty_r lemma

theories/examples/env_bisim.v
@@ -6,9 +6,11 @@ NB: This example was mentioned as open problem in Aleš's thesis.
 
 From stdpp Require Import namespaces.
 From iris.base_logic Require Import invariants na_invariants.
-From self.prelude Require Import base.
-From self.prob_lang Require Import notation proofmode primitive_laws.
+From self.prob_lang Require Import notation proofmode primitive_laws spec_rules.
 From self.logrel Require Import model rel_rules rel_tactics.
+From self.typing Require Import soundness.
+From self.prelude Require Import base.
+Set Default Proof Using "Type*".
 
 (* A diverging term. *)
 Definition Ω : expr := rec: "Ω" "v" := "Ω" "v".
@@ -21,31 +23,295 @@ Definition pchoice e1 e2 : expr :=
 Infix "⊕" := pchoice (at level 80) : expr_scope.
 
 Definition M : expr :=
-  if: !"x" = #0 then "x" <- #1 ;; #true else Ω.
+  if: !"x" = #0 then "x" <- #1 ;; #true else Ω #().
 
 Definition N : expr :=
-  if: !"x" = #0 then "x" <- #1 ;; #false else Ω.
+  if: !"x" = #0 then "x" <- #1 ;; #false else Ω #().
 
 Definition H : expr :=
   let: "x" := ref #0 in
+  let: "α" := #() in
+  (λ:<>, M ⊕ N).
+
+Definition H_with_tape : expr :=
+  let: "x" := ref #0 in
+  let: "α" := alloc in
   (λ:<>, M ⊕ N).
 
 Definition K : expr :=
   let: "x" := ref #0 in
+  let: "α" := #() in
   (λ:<>, M) ⊕ (λ:<>, N).
 
 Section proofs.
   Context `{!prelogrelGS Σ}.
-  Context `{!lockG Σ}.
 
   Definition bisimN := nroot.@"bisim".
 
-  Lemma HK :
-    ⊢ REL H << K : lrel_unit → lrel_bool.
+  Lemma H_with_tape_K_rel :
+    ⊢ REL H_with_tape << K : lrel_unit → lrel_bool.
+  Proof.
+    rewrite /H_with_tape /K.
+    rel_alloc_l x as "x". rel_alloc_r y as "y".
+    rel_pures_l. rel_pures_r.
+    rel_alloctape_l α as "α".
+    rel_bind_r (flip _)%E.
+    iApply (refines_couple_tape_flip with "[$α x y]"); [done|].
+    iIntros (b) "α /=".
+    rel_pures_l. rel_pures_r.
+    set (P := ((α ↪ [b] ∗ x ↦ #0 ∗ y ↦ₛ #0) ∨ (α ↪ [] ∗ x ↦ #1 ∗ y ↦ₛ #1))%I).
+    iApply (refines_na_alloc P bisimN).
+    iSplitL. 1: iModIntro ; iLeft ; iFrame.
+    iIntros "#Hinv".
+    destruct b.
+    (* Both cases are proven in *exactly* the same way. *)
+    - rel_pures_r.
+      rel_arrow_val.
+      iIntros (??) "_".
+      iApply (refines_na_inv with "[$Hinv]") ; [done|].
+      iIntros "[[(α & x & y) | (α & x & y)] Hclose]".
+      all: rel_pures_l ; rel_pures_r.
+      + rel_flip_l. rel_pures_l. rel_load_r. rel_load_l. rel_pures_l. rel_pures_r.
+        rel_store_l. rel_store_r. rel_pures_l. rel_pures_r.
+        iApply (refines_na_close with "[- $Hclose]").
+        iSplitL; [|rel_values].
+        iRight. iModIntro. iFrame.
+      + rel_load_r. rel_pures_r.
+        rel_apply_l refines_flip_empty_l.
+        iFrame. iIntros (b) "α".
+        destruct b.
+        (* Both cases are proven in *exactly* the same way. *)
+        * rel_pures_l. rel_load_l. rel_pures_l.
+          iApply (refines_na_close with "[- $Hclose]"). iSplitL.
+          1: { iModIntro. iRight. iFrame. }
+          rewrite refines_eq /refines_def.
+          iIntros (?) "??".
+          iLöb as "HH".
+          wp_rec.
+          now iApply ("HH" with "[$]").
+        * rel_pures_l. rel_load_l. rel_pures_l.
+          iApply (refines_na_close with "[- $Hclose]"). iSplitL.
+          1: iModIntro ; iRight ; iFrame.
+          rewrite refines_eq /refines_def.
+          iIntros (?) "??".
+          iLöb as "HH".
+          wp_rec.
+          now iApply ("HH" with "[$]").
+    - rel_pures_r.
+      rel_arrow_val.
+      iIntros (??) "_".
+      iApply (refines_na_inv with "[$Hinv]") ; [done|].
+      iIntros "[[(α & x & y) | (α & x & y)] Hclose]".
+      all: rel_pures_l ; rel_pures_r.
+      + rel_flip_l. rel_pures_l. rel_load_r. rel_load_l. rel_pures_l. rel_pures_r.
+        rel_store_l. rel_store_r. rel_pures_l. rel_pures_r.
+        iApply (refines_na_close with "[- $Hclose]").
+        iSplitL; [|rel_values].
+        iRight. iModIntro. iFrame.
+      + rel_load_r. rel_pures_r.
+        rel_apply_l refines_flip_empty_l.
+        iFrame. iIntros (b) "α".
+        destruct b.
+        (* Both cases are proven in *exactly* the same way. *)
+        * rel_pures_l. rel_load_l. rel_pures_l.
+          iApply (refines_na_close with "[- $Hclose]"). iSplitL.
+          1: { iModIntro. iRight. iFrame. }
+          rewrite refines_eq /refines_def.
+          iIntros (?) "??".
+          iLöb as "HH".
+          wp_rec.
+          now iApply ("HH" with "[$]").
+        * rel_pures_l. rel_load_l. rel_pures_l.
+          iApply (refines_na_close with "[- $Hclose]"). iSplitL.
+          1: iModIntro ; iRight ; iFrame.
+          rewrite refines_eq /refines_def.
+          iIntros (?) "??".
+          iLöb as "HH".
+          wp_rec.
+          now iApply ("HH" with "[$]").
+  Qed.
+
+  Lemma H_H_with_tape_rel :
+    ⊢ REL H << H_with_tape : lrel_unit → lrel_bool.
+  Proof.
+    rewrite /H_with_tape /H.
+    rel_alloc_l x as "x". rel_alloc_r y as "y".
+    rel_pures_l. rel_pures_r.
+    rel_alloctape_r α as "α".
+    rel_pures_r.
+    set (P := ((α ↪ₛ [] ∗ x ↦ #0 ∗ y ↦ₛ #0) ∨ (α ↪ₛ [] ∗ x ↦ #1 ∗ y ↦ₛ #1))%I).
+    iApply (refines_na_alloc P bisimN).
+    iSplitL. 1: iModIntro ; iLeft ; iFrame.
+    iIntros "#Hinv".
+    rel_arrow_val.
+    iIntros (??) "_".
+    iApply (refines_na_inv with "[$Hinv]") ; [done|].
+    iIntros "[[(α & x & y) | (α & x & y)] Hclose]".
+    all: rel_pures_l ; rel_pures_r.
+    + rel_bind_l (Flip _). rel_bind_r (Flip _).
+      rel_apply_l refines_couple_flips_r.
+      iFrame ; iIntros (b) "α".
+      destruct b.
+      * rel_pures_l. rel_pures_r. rel_load_l. rel_load_r. rel_pures_l. rel_pures_r.
+        rel_store_l. rel_store_r. rel_pures_l. rel_pures_r.
+        iApply (refines_na_close with "[- $Hclose]").
+        iSplitL; [|rel_values].
+        iRight ; iModIntro ; iFrame.
+      * rel_pures_l. rel_pures_r. rel_load_l. rel_load_r. rel_pures_l. rel_pures_r.
+        rel_store_l. rel_store_r. rel_pures_l. rel_pures_r.
+        iApply (refines_na_close with "[- $Hclose]").
+        iSplitL; [|rel_values].
+        iRight ; iModIntro ; iFrame.
+    + rel_bind_l (Flip _). rel_bind_r (Flip _).
+      rel_apply_l refines_couple_flips_r.
+      iFrame ; iIntros (b) "α".
+      destruct b.
+      * rel_pures_l. rel_pures_r. rel_load_l. rel_load_r. rel_pures_l. rel_pures_r.
+        iApply (refines_na_close with "[- $Hclose]"). iSplitL.
+        1: iModIntro ; iRight ; iFrame.
+        rewrite refines_eq /refines_def.
+        iIntros (?) "??".
+        iLöb as "HH".
+        wp_rec.
+        now iApply ("HH" with "[$]").
+      * rel_pures_l. rel_pures_r. rel_load_l. rel_load_r. rel_pures_l. rel_pures_r.
+        iApply (refines_na_close with "[- $Hclose]"). iSplitL.
+        1: iModIntro ; iRight ; iFrame.
+        rewrite refines_eq /refines_def.
+        iIntros (?) "??".
+        iLöb as "HH".
+        wp_rec.
+        now iApply ("HH" with "[$]").
+  Qed.
+
+
+  Lemma refines_flip_empty_r K E α A e :
+    to_val e = None →
+    α ↪ₛ [] ∗
+      (∀ (b : bool), α ↪ₛ [] -∗ REL e << fill K (Val #b) @ E : A)
+    ⊢ REL e << fill K (flip #lbl:α) @ E : A.
+  Proof.
+    iIntros (ev) "[Hα H]".
+    rewrite refines_eq /refines_def.
+    iIntros (K2) "[#Hs Hspec] Hnais /=".
   Admitted.
 
-  Lemma KH :
-    ⊢ REL H << K : lrel_unit → lrel_bool.
-  Admitted.
+  Lemma K_H_with_tape_rel :
+    ⊢ REL K << H_with_tape : lrel_unit → lrel_bool.
+  Proof.
+    rewrite /H_with_tape /K.
+    rel_alloc_l x as "x". rel_alloc_r y as "y".
+    rel_pures_l. rel_pures_r.
+    rel_alloctape_r α as "α".
+    rel_bind_l (flip _)%E.
+    iApply (refines_couple_flip_tape with "[$α x y]").
+    iIntros (b) "α /=".
+    rel_pures_l. rel_pures_r.
+    set (P := ((α ↪ₛ [b] ∗ x ↦ #0 ∗ y ↦ₛ #0) ∨ (α ↪ₛ [] ∗ x ↦ #1 ∗ y ↦ₛ #1))%I).
+    iApply (refines_na_alloc P bisimN).
+    iSplitL. 1: iModIntro ; iLeft ; iFrame.
+    iIntros "#Hinv".
+    destruct b.
+    (* Both cases are proven in *exactly* the same way. *)
+    - rel_pures_l.
+      rel_arrow_val.
+      iIntros (??) "_".
+      iApply (refines_na_inv with "[$Hinv]") ; [done|].
+      iIntros "[[(α & x & y) | (α & x & y)] Hclose]".
+      all: rel_pures_l ; rel_pures_r.
+      + rel_flip_r. rel_pures_r. rel_load_r. rel_load_l. rel_pures_l. rel_pures_r.
+        rel_store_l. rel_store_r. rel_pures_l. rel_pures_r.
+        iApply (refines_na_close with "[- $Hclose]").
+        iSplitL; [|rel_values].
+        iRight. iModIntro. iFrame.
+      + rel_load_l.
+        rel_apply_r refines_flip_empty_r. 1: auto.
+        iFrame. iIntros (b) "α". rel_pures_l.
+        destruct b.
+        (* Both cases are proven in *exactly* the same way. *)
+        all: rel_pures_r ; rel_load_r ; rel_pures_r ;
+          iApply (refines_na_close with "[- $Hclose]") ; iSplitL ;
+          [iModIntro ; iRight ; iFrame|] ;
+          rewrite refines_eq /refines_def ; iIntros (?) "??" ;
+          iLöb as "HH" ; wp_rec ; now iApply ("HH" with "[$]").
+    - rel_pures_l.
+      rel_arrow_val.
+      iIntros (??) "_".
+      iApply (refines_na_inv with "[$Hinv]") ; [done|].
+      iIntros "[[(α & x & y) | (α & x & y)] Hclose]".
+      all: rel_pures_l ; rel_pures_r.
+      + rel_flip_r. rel_pures_r. rel_load_r. rel_load_l. rel_pures_l. rel_pures_r.
+        rel_store_l. rel_store_r. rel_pures_l. rel_pures_r.
+        iApply (refines_na_close with "[- $Hclose]").
+        iSplitL; [|rel_values].
+        iRight. iModIntro. iFrame.
+      + rel_load_l.
+        rel_apply_r refines_flip_empty_r. 1: auto.
+        iFrame. iIntros (b) "α". rel_pures_l.
+        destruct b.
+        (* Both cases are proven in *exactly* the same way. *)
+        all: rel_pures_r ; rel_load_r ; rel_pures_r ;
+          iApply (refines_na_close with "[- $Hclose]") ; iSplitL ;
+          [iModIntro ; iRight ; iFrame|] ;
+          rewrite refines_eq /refines_def ; iIntros (?) "??" ;
+          iLöb as "HH" ; wp_rec ; now iApply ("HH" with "[$]").
+  Qed.
+
+  Lemma H_with_tape_H_rel :
+    ⊢ REL H_with_tape << H : lrel_unit → lrel_bool.
+  Proof.
+    rewrite /H_with_tape /H.
+    rel_alloc_l x as "x". rel_alloc_r y as "y".
+    rel_pures_l. rel_pures_r.
+    rel_alloctape_l α as "α".
+    rel_pures_r.
+    set (P := ((α ↪ [] ∗ x ↦ #0 ∗ y ↦ₛ #0) ∨ (α ↪ [] ∗ x ↦ #1 ∗ y ↦ₛ #1))%I).
+    iApply (refines_na_alloc P bisimN).
+    iSplitL. 1: iModIntro ; iLeft ; iFrame.
+    iIntros "#Hinv".
+    rel_arrow_val.
+    iIntros (??) "_".
+    iApply (refines_na_inv with "[$Hinv]") ; [done|].
+    iIntros "[[(α & x & y) | (α & x & y)] Hclose]".
+    all: rel_pures_l ; rel_pures_r.
+    + rel_bind_l (Flip _). rel_bind_r (Flip _).
+      rel_apply_l refines_couple_flips_l.
+      iFrame ; iIntros (b) "α".
+      destruct b ;
+        rel_pures_l ; rel_pures_r ; rel_load_l ; rel_load_r ; rel_pures_l ; rel_pures_r ;
+        rel_store_l ; rel_store_r ; rel_pures_l ; rel_pures_r ;
+        iApply (refines_na_close with "[- $Hclose]").
+      all: iSplitL; [|rel_values] ;
+        iRight ; iModIntro ; iFrame.
+    + rel_bind_l (Flip _). rel_bind_r (Flip _).
+      rel_apply_l refines_couple_flips_l.
+      iFrame ; iIntros (b) "α".
+      destruct b ;
+        rel_pures_l ; rel_pures_r ; rel_load_l ; rel_load_r ; rel_pures_l ; rel_pures_r ;
+        iApply (refines_na_close with "[- $Hclose]").
+        all: iSplitL ; [iModIntro ; iRight ; iFrame|] ;
+          rewrite refines_eq /refines_def ; iIntros (?) "??" ;
+          iLöb as "HH" ; wp_rec ; now iApply ("HH" with "[$]").
+  Qed.
 
 End proofs.
+
+Theorem H_K_refinement :
+  ∅ ⊨ H ≤ctx≤ K : () → TBool.
+Proof.
+  eapply ctx_refines_transitive.
+  - eapply (refines_sound prelogrelΣ).
+    intros. simpl. apply: H_H_with_tape_rel.
+  - eapply (refines_sound prelogrelΣ).
+    intros. apply: H_with_tape_K_rel.
+Qed.
+
+Theorem K_H_refinement :
+  ∅ ⊨ K ≤ctx≤ H : () → TBool.
+Proof.
+  eapply ctx_refines_transitive.
+  - eapply (refines_sound prelogrelΣ).
+    intros. simpl. apply: K_H_with_tape_rel.
+  - eapply (refines_sound prelogrelΣ).
+    intros. apply: H_with_tape_H_rel.
+Qed.
